src/RqRsMsgPred.v
@@ -173,6 +173,13 @@ Section PredMsg.
   
 End PredMsg.
 
+Definition AtomicMsgOutsInv {oifc} (mp: MsgOutPred oifc)
+           (boundf: list (Id Msg) (* inits *) ->
+                    list (Id Msg) (* eouts *)) :=
+  fun inits eouts st =>
+    SubList eouts (boundf inits) /\
+    Forall (fun eout => mp eout st.(bst_oss)) eouts.
+
 Section PredLock.
   Context {oifc: OStateIfc}.
   Variables (dtr: DTree)
